# Complete and Easy Let Bindings

In Complete and Easy, we have these rules:

    Γ  |-  e1 => A  -|  Θ      Θ  |-  [Θ]A•e2 ⇒⇒  C  -|  ∆
    ------------------------------------------------------- ->E
                    Γ  |-  e1 e2  -|  ∆

    Γ[α2^,α1^,α^=α1^->α2^],x:α1^  |-  e <= α2^  -|  ∆,x:α1^,∆'
    ------------------------------------------------------------------- ->1α (sec 8)
                 Γ[α^]  |-  \x. e <= α^  -|  ∆

    Γ,α^,β^,x:α^  |-  e <= β^  -|  ∆,x:α^,∆'
    ---------------------------------------- ->1=>
         Γ  |-  \x. e => α^ -> β^ -|  ∆

A let binding is just lambda and function application together:

    let y = e in b
    ==>
    (\y. b)e

So, the typing rule for a let binding should just be these rules run
one after another. First let's run `->E`:

    Γ  |-  (\y. b) => A  -|  Θ      Θ  |-  [Θ]A•e ⇒⇒  C  -|  ∆
    ----------------------------------------------------------- ->E (1)
                  Γ  |-  (\y. b) e => C  -|  ∆

Now, the top two need to be dealt with. Let's consider the one
on the left first.

    Γ,α^,β^,y:α^  |-  b <= β^  -|  Θ,y:α^,Θ'
    ------------------------------------------- ->I=> (2a)
         Γ  |-  \y. b => α^ -> β^  -|  Θ

Notice that this means that `A` from (1) is `α^ -> β^`. Next, we consider
the right side of the top of (1):

    
              Θ  |-  e <= [Θ]α^  -|  ∆
    ----------------------------------------- ->App (3a)
       Θ  |-  [Θ](α^ -> β^)•e ⇒⇒  C  -|  ∆

That's a pleasant simplification. All taken together, we have:

    Γ,α^,β^,y:α^  |-  b <= β^  -|  Θ,y:α^,Θ'      Θ  |-  e <= [Θ]α^  -|  ∆
    -------------------------------------------------------------------------- (4a)
                           Γ  |-  (\y. b) e => C  -|  ∆

I don't think that anything else can be squeezed out of this. One thing
is that if the no inference rule for abstraction from section 8 is used,
do we end up with the same rule for let bindings? Let's try it. We start
again with (1), but we will add a fresh `α^` to the context, and annotate
the lambda with it. I'm not totally sure if doing this is allowed:

    Γ,α^  |-  (\y. b) => A  -|  Θ      Θ  |-  [Θ]A•e ⇒⇒  C  -|  ∆
    -------------------------------------------------------------- ->E (1)
                  Γ  |-  (\y. b) e => C  -|  ∆

But now we use `->1α` for abstraction:

    Γ,α2^,α1^,α=α1^->α2^,y:α1^  |-  b <= α2^  -|  Θ,y:α1^,Θ'
    ----------------------------------------------------------- ->1α (2b)
                 Γ,α^  |-  \y. b <= α^  -|  Θ
    ----------------------------------------------------------- Anno
             Γ,α^  |-  ((\y. b) : α^) => α^  -|  Θ

This time, `A` from (1) is `α^`, but the substitution under `Θ`,
means that `A` is replaced by `α1^->α2^`. So, we again apply
rule `->App` to the top right part of (1):

              Θ  |-  e <= [Θ]α1^  -|  ∆
    ----------------------------------------- ->App (3b)
       Θ  |-  [Θ](α1^ -> α2^)•e ⇒⇒  C  -|  ∆

Taken all together, we have:


    Γ,α2^,α1^,α=α1^->α2^,y:α1^  |-  b <= α2^  -|  Θ,y:α1^,Θ'      Θ  |-  e <= [Θ]α1^  -|  ∆
    ----------------------------------------------------------------------------------------- (4b)
                           Γ  |-  (\y. b) e => C  -|  ∆

Since `α` is solved, it can be removed, and that makes (4b) essentially
the same rule as (4a).

This is all good and well. I have discovered, however, that in a variant of
this system with kind constant (no existentials for kinds), this does not
work. The problem is that in the variant, I use the no-inference rule precisely
because it never extends the context with existentials. However, to massage
the expression enough to get `Anno` in work in (2b), I had to extend the
context, adding `Γ,α^`, which is a problem. Although such a rule is not
derivable, I wonder if I may extend the no-inference variant of
Complete and Easy with this:

    Γ  |-  e => A  -|  Θ       Θ,y:[Θ]A  |-  b => C  -|  ∆,y
    -------------------------------------------------------- (Bonus)
            Γ  |-  (let y = e in b) => C  -|  ∆

Interesting, but I do not know if it destroys any of the properties of the
system. It is pretty heavy on type synthesis. Notably, it processes things
in the opposite order of the derivable rule. That is, in `Bonus`, we
synthesize the type of `e` first. In (4a), we check `b` against a type
first.
